feat(*) cleaner wellorder theorem + order setups

HOTG/Binary_Relations/Properties/HOTG_Binary_Relations_Antisymmetric.thy
@@ -8,11 +8,13 @@ overloading
   antisymmetric_on_set \<equiv> "antisymmetric_on :: set \<Rightarrow> (set \<Rightarrow> set \<Rightarrow> bool) \<Rightarrow> bool"
   set_antisymmetric_on_pred \<equiv> "antisymmetric_on :: (set \<Rightarrow> bool) \<Rightarrow> set \<Rightarrow> bool"
   set_antisymmetric_on_set \<equiv> "antisymmetric_on :: set \<Rightarrow> set \<Rightarrow> bool"
+  antisymmetric_set \<equiv> "antisymmetric :: set \<Rightarrow> bool"
 begin
   definition "antisymmetric_on_set (A :: set) (R :: set \<Rightarrow> set \<Rightarrow> bool) \<equiv>
     antisymmetric_on (mem_of A) R"
   definition "set_antisymmetric_on_pred (P :: set \<Rightarrow> bool) (R :: set) \<equiv> antisymmetric_on P (rel R)"
   definition "set_antisymmetric_on_set (A :: set) (R :: set) \<equiv> antisymmetric_on (mem_of A) R"
+  definition "antisymmetric_set :: set \<Rightarrow> bool \<equiv> antisymmetric_on (\<top> :: set \<Rightarrow> bool)"
 end
 
 lemma antisymmetric_on_set_eq_antisymmetric_on_pred [simp]:
@@ -34,7 +36,8 @@ lemma set_antisymmetric_on_pred_iff_antisymmetric_on_pred [iff]:
 
 lemma set_antisymmetric_on_pred_iff_antisymmetric_on_pred_uhint [uhint]:
   assumes "R \<equiv> rel S"
-  shows "antisymmetric_on (P :: set \<Rightarrow> bool) S \<equiv> antisymmetric_on P R"
+  and "P :: set \<Rightarrow> bool \<equiv> P'"
+  shows "antisymmetric_on P S \<equiv> antisymmetric_on P' R"
   using assms by simp
 
 lemma set_antisymmetric_on_set_eq_set_antisymmetric_on_pred [simp]:
@@ -50,6 +53,20 @@ lemma set_antisymmetric_on_set_iff_set_antisymmetric_on_pred [iff]:
   "antisymmetric_on (S :: set) (R :: set) \<longleftrightarrow> antisymmetric_on (mem_of S) R"
   by simp
 
+lemma antisymmetric_set_eq_set_antisymmetric_on:
+  "(antisymmetric :: set \<Rightarrow> _) = antisymmetric_on (\<top> :: set \<Rightarrow> bool)"
+  unfolding antisymmetric_set_def ..
 
+lemma antisymmetric_set_eq_set_antisymmetric_on_uhint [uhint]:
+  "P \<equiv> (\<top> :: set \<Rightarrow> bool) \<Longrightarrow> (antisymmetric :: set \<Rightarrow> _) \<equiv> antisymmetric_on P"
+  by (simp add: antisymmetric_set_eq_set_antisymmetric_on)
+
+lemma antisymmetric_set_iff_antisymmetric_pred [iff]:
+  "antisymmetric S \<longleftrightarrow> antisymmetric (rel S)"
+  unfolding antisymmetric_set_eq_set_antisymmetric_on by (urule refl)
+
+lemma antisymmetric_set_eq_antisymmetric_pred_uhint [uhint]:
+  "R \<equiv> rel A \<Longrightarrow> antisymmetric A \<equiv> antisymmetric R"
+  by simp
 
 end
