HOTG/Binary_Relations/Properties/HOTG_Binary_Relations_Injective.thy
@@ -10,11 +10,13 @@ overloading
   rel_injective_on_set \<equiv> "rel_injective_on :: set \<Rightarrow> (set \<Rightarrow> 'a \<Rightarrow> bool) \<Rightarrow> bool"
   set_rel_injective_on_pred \<equiv> "rel_injective_on :: (set \<Rightarrow> bool) \<Rightarrow> set \<Rightarrow> bool"
   set_rel_injective_on_set \<equiv> "rel_injective_on :: set \<Rightarrow> set \<Rightarrow> bool"
+  rel_injective_set \<equiv> "rel_injective :: set \<Rightarrow> bool"
 begin
   definition "rel_injective_on_set (A :: set) (R :: set \<Rightarrow> 'a \<Rightarrow> bool) \<equiv>
     rel_injective_on (mem_of A) R"
   definition "set_rel_injective_on_pred (P :: set \<Rightarrow> bool) (R :: set) \<equiv> rel_injective_on P (rel R)"
   definition "set_rel_injective_on_set (A :: set) (R :: set) \<equiv> rel_injective_on (mem_of A) R"
+  definition "rel_injective_set :: set \<Rightarrow> bool \<equiv> rel_injective_on (\<top> :: set \<Rightarrow> bool)"
 end
 
 lemma rel_injective_on_set_eq_rel_injective_on_pred [simp]:
@@ -36,7 +38,8 @@ lemma set_rel_injective_on_pred_iff_rel_injective_on_pred [iff]:
 
 lemma set_rel_injective_on_pred_iff_rel_injective_on_pred_uhint [uhint]:
   assumes "R \<equiv> rel S"
-  shows "rel_injective_on (P :: set \<Rightarrow> bool) S \<equiv> rel_injective_on P R"
+  and "P :: set \<Rightarrow> bool \<equiv> P'"
+  shows "rel_injective_on P S \<equiv> rel_injective_on P' R"
   using assms by simp
 
 lemma set_rel_injective_on_set_eq_set_rel_injective_on_pred [simp]:
@@ -83,7 +86,8 @@ lemma set_rel_injective_at_pred_iff_rel_injective_at_pred [iff]:
 
 lemma set_rel_injective_at_pred_iff_rel_injective_at_pred_uhint [uhint]:
   assumes "R \<equiv> rel S"
-  shows "rel_injective_at (P :: set \<Rightarrow> bool) S \<equiv> rel_injective_at P R"
+  and "P :: set \<Rightarrow> bool \<equiv> P'"
+  shows "rel_injective_at P S \<equiv> rel_injective_at P' R"
   using assms by simp
 
 lemma set_rel_injective_at_set_eq_set_rel_injective_at_pred [simp]:
@@ -99,5 +103,20 @@ lemma set_rel_injective_at_set_iff_set_rel_injective_at_pred [iff]:
   "rel_injective_at (S :: set) (R :: set) \<longleftrightarrow> rel_injective_at (mem_of S) R"
   by simp
 
+lemma rel_injective_set_eq_set_rel_injective_on:
+  "(rel_injective :: set \<Rightarrow> _) = rel_injective_on (\<top> :: set \<Rightarrow> bool)"
+  unfolding rel_injective_set_def ..
+
+lemma rel_injective_set_eq_set_rel_injective_on_uhint [uhint]:
+  "P \<equiv> (\<top> :: set \<Rightarrow> bool) \<Longrightarrow> (rel_injective :: set \<Rightarrow> _) \<equiv> rel_injective_on P"
+  by (simp add: rel_injective_set_eq_set_rel_injective_on)
+
+lemma rel_injective_set_iff_rel_injective_pred [iff]:
+  "rel_injective S \<longleftrightarrow> rel_injective (rel S)"
+  unfolding rel_injective_set_eq_set_rel_injective_on by (urule refl)
+
+lemma rel_injective_set_eq_rel_injective_pred_uhint [uhint]:
+  "R \<equiv> rel A \<Longrightarrow> rel_injective A \<equiv> rel_injective R"
+  by simp
 
 end
