HOTG/Binary_Relations/Properties/HOTG_Binary_Relations_Reflexive.thy
@@ -10,10 +10,12 @@ overloading
   reflexive_on_set \<equiv> "reflexive_on :: set \<Rightarrow> (set \<Rightarrow> set \<Rightarrow> bool) \<Rightarrow> bool"
   set_reflexive_on_pred \<equiv> "reflexive_on :: (set \<Rightarrow> bool) \<Rightarrow> set \<Rightarrow> bool"
   set_reflexive_on_set \<equiv> "reflexive_on :: set \<Rightarrow> set \<Rightarrow> bool"
+  reflexive_set \<equiv> "reflexive :: set \<Rightarrow> bool"
 begin
   definition "reflexive_on_set (A :: set) :: (set \<Rightarrow> set \<Rightarrow> bool) \<Rightarrow> bool \<equiv> reflexive_on (mem_of A)"
   definition "set_reflexive_on_pred (P :: set \<Rightarrow> bool) (R :: set) \<equiv> reflexive_on P (rel R)"
   definition "set_reflexive_on_set (A :: set) (R :: set) \<equiv> reflexive_on (mem_of A) R"
+  definition "reflexive_set :: set \<Rightarrow> bool \<equiv> reflexive_on (\<top> :: set \<Rightarrow> bool)"
 end
 
 lemma reflexive_on_set_eq_reflexive_on_pred [simp]:
@@ -35,7 +37,8 @@ lemma set_reflexive_on_pred_iff_reflexive_on_pred [iff]:
 
 lemma set_reflexive_on_pred_iff_reflexive_on_pred_uhint [uhint]:
   assumes "R \<equiv> rel S"
-  shows "reflexive_on (P :: set \<Rightarrow> bool) S \<equiv> reflexive_on P R"
+  and "P :: set \<Rightarrow> bool \<equiv> P'"
+  shows "reflexive_on P S \<equiv> reflexive_on P' R"
   using assms by simp
 
 lemma set_reflexive_on_set_eq_set_reflexive_on_pred [simp]:
@@ -51,5 +54,20 @@ lemma set_reflexive_on_set_iff_set_reflexive_on_pred [iff]:
   "reflexive_on (S :: set) (R :: set) \<longleftrightarrow> reflexive_on (mem_of S) R"
   by simp
 
+lemma reflexive_set_eq_set_reflexive_on:
+  "(reflexive :: set \<Rightarrow> _) = reflexive_on (\<top> :: set \<Rightarrow> bool)"
+  unfolding reflexive_set_def ..
+
+lemma reflexive_set_eq_set_reflexive_on_uhint [uhint]:
+  "P \<equiv> (\<top> :: set \<Rightarrow> bool) \<Longrightarrow> (reflexive :: set \<Rightarrow> _) \<equiv> reflexive_on P"
+  by (simp add: reflexive_set_eq_set_reflexive_on)
+
+lemma reflexive_set_iff_reflexive_pred [iff]:
+  "reflexive S \<longleftrightarrow> reflexive (rel S)"
+  unfolding reflexive_set_eq_set_reflexive_on by (urule refl)
+
+lemma reflexive_set_eq_reflexive_pred_uhint [uhint]:
+  "R \<equiv> rel A \<Longrightarrow> reflexive A \<equiv> reflexive R"
+  by simp
 
 end
