HOTG/Binary_Relations/Properties/HOTG_Binary_Relations_Wellfounded.thy
@@ -7,18 +7,68 @@ theory HOTG_Binary_Relations_Wellfounded
 begin
 
 overloading
+  wellfounded_on_set \<equiv> "wellfounded_on :: set \<Rightarrow> (set \<Rightarrow> set \<Rightarrow> bool) \<Rightarrow> bool"
+  set_wellfounded_on_pred \<equiv> "wellfounded_on :: (set \<Rightarrow> bool) \<Rightarrow> set \<Rightarrow> bool"
+  set_wellfounded_on_set \<equiv> "wellfounded_on :: set \<Rightarrow> set \<Rightarrow> bool"
   wellfounded_set \<equiv> "wellfounded :: set \<Rightarrow> bool"
 begin
-  definition "wellfounded_set (R :: set) \<equiv> wellfounded (rel R)"
+  definition "wellfounded_on_set (A :: set) (R :: set \<Rightarrow> set \<Rightarrow> bool) \<equiv>
+    wellfounded_on (mem_of A) R"
+  definition "set_wellfounded_on_pred (P :: set \<Rightarrow> bool) (R :: set) \<equiv> wellfounded_on P (rel R)"
+  definition "set_wellfounded_on_set (A :: set) (R :: set) \<equiv> wellfounded_on (mem_of A) R"
+  definition "wellfounded_set :: set \<Rightarrow> bool \<equiv> wellfounded_on (\<top> :: set \<Rightarrow> bool)"
 end
 
-lemma wellfounded_set_iff_wellfounded_rel [iff]:
-  "wellfounded R \<longleftrightarrow> wellfounded (rel R)"
-  unfolding wellfounded_set_def by simp
+lemma wellfounded_on_set_eq_wellfounded_on_pred [simp]:
+  "(wellfounded_on (S :: set) :: (set \<Rightarrow> set \<Rightarrow> bool) \<Rightarrow> bool) = wellfounded_on (mem_of S)"
+  unfolding wellfounded_on_set_def by simp
 
-lemma set_wellfounded_pred_iff_wellfounded_pred_uhint [uhint]:
-  assumes "R \<equiv> rel S"
-  shows "wellfounded S \<equiv> wellfounded R"
+lemma wellfounded_on_set_eq_wellfounded_on_pred_uhint [uhint]:
+  assumes "P \<equiv> mem_of S"
+  shows "wellfounded_on (S :: set) :: (set \<Rightarrow> set \<Rightarrow> bool) \<Rightarrow> bool \<equiv> wellfounded_on P"
   using assms by simp
+
+lemma wellfounded_on_set_iff_wellfounded_on_pred [iff]:
+  "wellfounded_on (S :: set) (R :: set \<Rightarrow> set \<Rightarrow> bool) \<longleftrightarrow> wellfounded_on (mem_of S) R"
+  by simp
+
+lemma set_wellfounded_on_pred_iff_wellfounded_on_pred [iff]:
+  "wellfounded_on (P :: set \<Rightarrow> bool) R \<longleftrightarrow> wellfounded_on P (rel R)"
+  unfolding set_wellfounded_on_pred_def by simp
+
+lemma set_wellfounded_on_pred_iff_wellfounded_on_pred_uhint [uhint]:
+  assumes "R \<equiv> rel S"
+  and "P :: set \<Rightarrow> bool \<equiv> P'"
+  shows "wellfounded_on P S \<equiv> wellfounded_on P' R"
+  using assms by simp
+
+lemma set_wellfounded_on_set_eq_set_wellfounded_on_pred [simp]:
+  "(wellfounded_on (S :: set) :: set \<Rightarrow> bool) = wellfounded_on (mem_of S)"
+  unfolding set_wellfounded_on_set_def by simp
+
+lemma set_wellfounded_on_set_eq_set_wellfounded_on_pred_uhint [uhint]:
+  assumes "P \<equiv> mem_of S"
+  shows "wellfounded_on (S :: set) :: set \<Rightarrow> bool \<equiv> wellfounded_on P"
+  using assms by simp
+
+lemma set_wellfounded_on_set_iff_set_wellfounded_on_pred [iff]:
+  "wellfounded_on (S :: set) (R :: set) \<longleftrightarrow> wellfounded_on (mem_of S) R"
+  by simp
+
+lemma wellfounded_set_eq_set_wellfounded_on:
+  "(wellfounded :: set \<Rightarrow> _) = wellfounded_on (\<top> :: set \<Rightarrow> bool)"
+  unfolding wellfounded_set_def ..
+
+lemma wellfounded_set_eq_set_wellfounded_on_uhint [uhint]:
+  "P \<equiv> (\<top> :: set \<Rightarrow> bool) \<Longrightarrow> (wellfounded :: set \<Rightarrow> _) \<equiv> wellfounded_on P"
+  by (simp add: wellfounded_set_eq_set_wellfounded_on)
+
+lemma wellfounded_set_iff_wellfounded_pred [iff]:
+  "wellfounded S \<longleftrightarrow> wellfounded (rel S)"
+  unfolding wellfounded_set_eq_set_wellfounded_on by (urule refl)
+
+lemma wellfounded_set_eq_wellfounded_pred_uhint [uhint]:
+  "R \<equiv> rel A \<Longrightarrow> wellfounded A \<equiv> wellfounded R"
+  by simp
 
 end
