HOTG/Binary_Relations/Recursions/HOTG_Epsilon_Recursion.thy
@@ -1,7 +1,7 @@
 \<^marker>\<open>creator "Kevin Kappelmann"\<close>
 \<^marker>\<open>creator "Niklas Krofta"\<close>
-section \<open>Transfinite Recursion\<close>
-theory HOTG_Transfinite_Recursion
+section \<open>Epsilon Recursion\<close>
+theory HOTG_Epsilon_Recursion
   imports
     HOTG_Less_Than
     HOTG_Functions_Restrict
@@ -14,16 +14,16 @@ context
   includes fun_restrict_syntax no_rel_restrict_syntax
 begin
 
-definition transfrec :: "((set \<Rightarrow> 'a) \<Rightarrow> set \<Rightarrow> 'a) \<Rightarrow> set \<Rightarrow> 'a" where
-  "transfrec step = wftrec (<) (\<lambda>f X. step f\<restriction>\<^bsub>X\<^esub> X)"
+definition mem_rec :: "((set \<Rightarrow> 'a) \<Rightarrow> set \<Rightarrow> 'a) \<Rightarrow> set \<Rightarrow> 'a" where
+  "mem_rec step = wft_rec (<) (\<lambda>f X. step f\<restriction>\<^bsub>X\<^esub> X)"
 
-corollary transfrec_eq: "transfrec step X = step (transfrec step)\<restriction>\<^bsub>X\<^esub> X"
+corollary mem_rec_eq: "mem_rec step X = step (mem_rec step)\<restriction>\<^bsub>X\<^esub> X"
 proof -
   have fun_rel_restrict_eq: "(fun_rel_restrict f (<) X)\<restriction>\<^bsub>X\<^esub> = f\<restriction>\<^bsub>X\<^esub>" for f
     using lt_if_mem by (auto simp: fun_restrict_eq_if)
-  then have "transfrec step X = step ((fun_rel_restrict (transfrec step) (<) X)\<restriction>\<^bsub>X\<^esub>) X"
+  then have "mem_rec step X = step ((fun_rel_restrict (mem_rec step) (<) X)\<restriction>\<^bsub>X\<^esub>) X"
     using wellfounded_lt transitive_lt
-    by (simp_all only: wfrec_step_eq wftrec_eq_wfrec_stepI transfrec_def)
+    by (simp only: wf_rec_step_eq wft_rec_eq_wf_rec_stepI mem_rec_def)
   then show ?thesis unfolding fun_rel_restrict_eq by simp
 qed
 
