HOTG/Binary_Relations/HOTG_Binary_Relations.thy
@@ -2,13 +2,13 @@
 theory HOTG_Binary_Relations
   imports
     HOTG_Binary_Relation_Properties
-    HOTG_Transfinite_Recursion
+    HOTG_Epsilon_Recursion
+    HOTG_Wellfounded_Recursion
     HOTG_Binary_Relation_Functions
     HOTG_Binary_Relations_Agree
     HOTG_Binary_Relations_Base
     HOTG_Binary_Relations_Extend
     HOTG_Binary_Relations_Pow
-    HOTG_Binary_Relation_Isomorphism
 begin
 
 
