HOTG/Binary_Relations/Properties/HOTG_Binary_Relation_Properties.thy
@@ -3,6 +3,7 @@ subsection \<open>Basic Properties\<close>
 theory HOTG_Binary_Relation_Properties
   imports
     HOTG_Binary_Relations_Antisymmetric
+    HOTG_Binary_Relations_Asymmetric
     HOTG_Binary_Relations_Connected
     HOTG_Binary_Relations_Injective
     HOTG_Binary_Relations_Irreflexive
@@ -13,7 +14,6 @@ theory HOTG_Binary_Relation_Properties
     HOTG_Binary_Relations_Symmetric
     HOTG_Binary_Relations_Transitive
     HOTG_Binary_Relations_Wellfounded
-    HOTG_Binary_Relations_Wellorder
 begin
 
 end
