HOTG/Binary_Relations/Recursions/HOTG_Wellfounded_Recursion.thy
@@ -1,0 +1,22 @@
+\<^marker>\<open>creator "Kevin Kappelmann"\<close>
+subsection \<open>Well-Founded Recursion\<close>
+theory HOTG_Wellfounded_Recursion
+  imports
+    HOTG_Basics
+    Transport.Wellfounded_Recursion
+begin
+
+definition "wf_rec_on_set (A :: set) :: (set \<Rightarrow> set \<Rightarrow> bool) \<Rightarrow> ((set \<Rightarrow> 'a) \<Rightarrow> set \<Rightarrow> 'a) \<Rightarrow> set \<Rightarrow> 'a
+  \<equiv> wf_rec_on (mem_of A)"
+adhoc_overloading wf_rec_on wf_rec_on_set
+
+lemma wf_rec_on_set_eq_wf_rec_on_pred [simp]: "wf_rec_on A = wf_rec_on (mem_of A)"
+  unfolding wf_rec_on_set_def by auto
+
+lemma wf_rec_on_set_eq_wf_rec_on_pred_uhint [uhint]:
+  assumes "P \<equiv> mem_of A"
+  shows "wf_rec_on A \<equiv> wf_rec_on (mem_of A)"
+  using assms wf_rec_on_set_eq_wf_rec_on_pred by simp
+
+
+end
