HOTG/Orders/HOTG_Order_Isomorphisms.thy
@@ -1,0 +1,43 @@
+\<^marker>\<open>creator "Kevin Kappelmann"\<close>
+\<^marker>\<open>creator "Niklas Krofa"\<close>
+theory HOTG_Order_Isomorphisms
+  imports
+    HOTG_Basics
+    Transport.Order_Isomorphisms
+begin
+
+definition "order_isomorphism_on_set A B \<equiv> order_isomorphism_on (mem_of A) (mem_of B)"
+adhoc_overloading order_isomorphism_on order_isomorphism_on_set
+
+lemma order_isomorphism_on_set_eq_order_isomorphism_on_pred [simp]:
+  "order_isomorphism_on A B = order_isomorphism_on (mem_of A) (mem_of B)"
+  unfolding order_isomorphism_on_set_def by simp
+
+lemma order_isomorphism_on_set_eq_order_isomorphism_on_pred_uhint [uhint]:
+  assumes "P \<equiv> mem_of A"
+  and "Q \<equiv> mem_of B"
+  shows "order_isomorphism_on A B \<equiv> order_isomorphism_on P Q"
+  using assms by simp
+
+lemma order_isomorphism_on_set_iff_order_isomorphism_on_pred [iff]:
+  "order_isomorphism_on A B L R l r \<longleftrightarrow> order_isomorphism_on (mem_of A) (mem_of B) L R l r"
+  by simp
+
+definition "order_isomorphic_on_set A B = order_isomorphic_on (mem_of A) (mem_of B)"
+adhoc_overloading order_isomorphic_on order_isomorphic_on_set
+
+lemma order_isomorphic_on_set_eq_order_isomorphic_on_pred [simp]:
+  "order_isomorphic_on A B = order_isomorphic_on (mem_of A) (mem_of B)"
+  unfolding order_isomorphic_on_set_def by simp
+
+lemma order_isomorphic_on_set_eq_order_isomorphic_on_pred_uhint [uhint]:
+  assumes "P \<equiv> mem_of A"
+  and "Q \<equiv> mem_of B"
+  shows "order_isomorphic_on A B \<equiv> order_isomorphic_on P Q"
+  using assms by simp
+
+lemma order_isomorphic_on_set_iff_order_isomorphic_on_pred [iff]:
+  "order_isomorphic_on A B L R \<longleftrightarrow> order_isomorphic_on (mem_of A) (mem_of B) L R"
+  by simp
+
+end
