HOTG/Orders/HOTG_Partial_Equivalence_Relations.thy
@@ -1,0 +1,71 @@
+\<^marker>\<open>creator "Kevin Kappelmann"\<close>
+subsection \<open>Partial Equivalence Relations\<close>
+theory HOTG_Partial_Equivalence_Relations
+  imports
+    HOTG_Binary_Relations_Symmetric
+    HOTG_Binary_Relations_Transitive
+    Transport.Partial_Equivalence_Relations
+begin
+
+lemma partial_equivalence_rel_on_set_eq_partial_equivalence_rel_on_pred [simp]:
+  "(partial_equivalence_rel_on (S :: set) :: (set \<Rightarrow> set \<Rightarrow> bool) \<Rightarrow> bool) = partial_equivalence_rel_on (mem_of S)"
+  unfolding partial_equivalence_rel_on_def by simp
+
+lemma partial_equivalence_rel_on_set_eq_partial_equivalence_rel_on_pred_uhint [uhint]:
+  assumes "P \<equiv> mem_of S"
+  shows "partial_equivalence_rel_on (S :: set) :: (set \<Rightarrow> set \<Rightarrow> bool) \<Rightarrow> bool \<equiv> partial_equivalence_rel_on P"
+  using assms by simp
+
+lemma partial_equivalence_rel_on_set_iff_partial_equivalence_rel_on_pred [iff]:
+  "partial_equivalence_rel_on (S :: set) (R :: set \<Rightarrow> set \<Rightarrow> bool) \<longleftrightarrow> partial_equivalence_rel_on (mem_of S) R"
+  by simp
+
+lemma set_partial_equivalence_rel_on_pred_iff_partial_equivalence_rel_on_pred [iff]:
+  "partial_equivalence_rel_on (P :: set \<Rightarrow> bool) R \<longleftrightarrow> partial_equivalence_rel_on P (rel R)"
+  unfolding partial_equivalence_rel_on_def by simp
+
+lemma set_partial_equivalence_rel_on_pred_iff_partial_equivalence_rel_on_pred_uhint [uhint]:
+  assumes "R \<equiv> rel S"
+  and "P :: set \<Rightarrow> bool \<equiv> P'"
+  shows "partial_equivalence_rel_on P S \<equiv> partial_equivalence_rel_on P' R"
+  using assms by simp
+
+lemma set_partial_equivalence_rel_on_set_eq_set_partial_equivalence_rel_on_pred [simp]:
+  "(partial_equivalence_rel_on (S :: set) :: set \<Rightarrow> bool) = partial_equivalence_rel_on (mem_of S)"
+  unfolding partial_equivalence_rel_on_def by simp
+
+lemma set_partial_equivalence_rel_on_set_eq_set_partial_equivalence_rel_on_pred_uhint [uhint]:
+  assumes "P \<equiv> mem_of S"
+  shows "partial_equivalence_rel_on (S :: set) :: set \<Rightarrow> bool \<equiv> partial_equivalence_rel_on P"
+  using assms by simp
+
+lemma set_partial_equivalence_rel_on_set_iff_set_partial_equivalence_rel_on_pred [iff]:
+  "partial_equivalence_rel_on (S :: set) (R :: set) \<longleftrightarrow> partial_equivalence_rel_on (mem_of S) R"
+  by simp
+
+overloading
+  partial_equivalence_rel_set \<equiv> "partial_equivalence_rel :: set \<Rightarrow> bool"
+begin
+  definition "(partial_equivalence_rel_set :: set \<Rightarrow> bool) \<equiv>
+    partial_equivalence_rel_on (\<top> :: set \<Rightarrow> bool)"
+end
+
+lemma partial_equivalence_rel_set_eq_partial_equivalence_rel_on:
+  "(partial_equivalence_rel :: set \<Rightarrow> bool) = partial_equivalence_rel_on (\<top> :: set \<Rightarrow> bool)"
+  unfolding partial_equivalence_rel_set_def ..
+
+lemma partial_equivalence_rel_set_eq_partial_equivalence_rel_on_uhint [uhint]:
+  assumes "P \<equiv> \<top> :: set \<Rightarrow> bool"
+  shows "(partial_equivalence_rel :: set \<Rightarrow> bool) \<equiv> partial_equivalence_rel_on P"
+  using assms by (simp add: partial_equivalence_rel_set_eq_partial_equivalence_rel_on)
+
+lemma partial_equivalence_rel_set_iff_partial_equivalence_rel_pred [iff]:
+  "partial_equivalence_rel S \<longleftrightarrow> partial_equivalence_rel (rel S)"
+  unfolding partial_equivalence_rel_set_def by (urule refl)
+
+lemma partial_equivalence_rel_set_iff_partial_equivalence_rel_pred_uhint [uhint]:
+  assumes "R \<equiv> rel S"
+  shows "partial_equivalence_rel S \<equiv> partial_equivalence_rel R"
+  using assms by simp
+
+end
