HOTG/Orders/HOTG_Preorders.thy
@@ -1,0 +1,69 @@
+\<^marker>\<open>creator "Kevin Kappelmann"\<close>
+subsection \<open>Preorders\<close>
+theory HOTG_Preorders
+  imports
+    HOTG_Binary_Relations_Reflexive
+    HOTG_Binary_Relations_Transitive
+    Transport.Preorders
+begin
+
+lemma preorder_on_set_eq_preorder_on_pred [simp]:
+  "(preorder_on (S :: set) :: (set \<Rightarrow> set \<Rightarrow> bool) \<Rightarrow> bool) = preorder_on (mem_of S)"
+  unfolding preorder_on_def by simp
+
+lemma preorder_on_set_eq_preorder_on_pred_uhint [uhint]:
+  assumes "P \<equiv> mem_of S"
+  shows "preorder_on (S :: set) :: (set \<Rightarrow> set \<Rightarrow> bool) \<Rightarrow> bool \<equiv> preorder_on P"
+  using assms by simp
+
+lemma preorder_on_set_iff_preorder_on_pred [iff]:
+  "preorder_on (S :: set) (R :: set \<Rightarrow> set \<Rightarrow> bool) \<longleftrightarrow> preorder_on (mem_of S) R"
+  by simp
+
+lemma set_preorder_on_pred_iff_preorder_on_pred [iff]:
+  "preorder_on (P :: set \<Rightarrow> bool) R \<longleftrightarrow> preorder_on P (rel R)"
+  unfolding preorder_on_def by simp
+
+lemma set_preorder_on_pred_iff_preorder_on_pred_uhint [uhint]:
+  assumes "R \<equiv> rel S"
+  and "P :: set \<Rightarrow> bool \<equiv> P'"
+  shows "preorder_on P S \<equiv> preorder_on P' R"
+  using assms by simp
+
+lemma set_preorder_on_set_eq_set_preorder_on_pred [simp]:
+  "(preorder_on (S :: set) :: set \<Rightarrow> bool) = preorder_on (mem_of S)"
+  unfolding preorder_on_def by simp
+
+lemma set_preorder_on_set_eq_set_preorder_on_pred_uhint [uhint]:
+  assumes "P \<equiv> mem_of S"
+  shows "preorder_on (S :: set) :: set \<Rightarrow> bool \<equiv> preorder_on P"
+  using assms by simp
+
+lemma set_preorder_on_set_iff_set_preorder_on_pred [iff]:
+  "preorder_on (S :: set) (R :: set) \<longleftrightarrow> preorder_on (mem_of S) R"
+  by simp
+
+overloading
+  preorder_set \<equiv> "preorder :: set \<Rightarrow> bool"
+begin
+  definition "(preorder_set :: set \<Rightarrow> bool) \<equiv> preorder_on (\<top> :: set \<Rightarrow> bool)"
+end
+
+lemma preorder_set_eq_preorder_on:
+  "(preorder :: set \<Rightarrow> bool) = preorder_on (\<top> :: set \<Rightarrow> bool)"
+  unfolding preorder_set_def ..
+
+lemma preorder_set_eq_preorder_on_uhint [uhint]:
+  assumes "P \<equiv> \<top> :: set \<Rightarrow> bool"
+  shows "(preorder :: set \<Rightarrow> bool) \<equiv> preorder_on P"
+  using assms by (simp add: preorder_set_eq_preorder_on)
+
+lemma preorder_set_iff_preorder_pred [iff]: "preorder S \<longleftrightarrow> preorder (rel S)"
+  unfolding preorder_set_def by (urule refl)
+
+lemma preorder_set_iff_preorder_pred_uhint [uhint]:
+  assumes "R \<equiv> rel S"
+  shows "preorder S \<equiv> preorder R"
+  using assms by simp
+
+end
