HOTG/Orders/HOTG_Strict_Partial_Orders.thy
@@ -1,0 +1,70 @@
+\<^marker>\<open>creator "Kevin Kappelmann"\<close>
+subsection \<open>Strict Partial Orders\<close>
+theory HOTG_Strict_Partial_Orders
+  imports
+    HOTG_Binary_Relations_Asymmetric
+    HOTG_Binary_Relations_Transitive
+    Transport.Strict_Partial_Orders
+begin
+
+lemma strict_partial_order_on_set_eq_strict_partial_order_on_pred [simp]:
+  "(strict_partial_order_on (S :: set) :: (set \<Rightarrow> set \<Rightarrow> bool) \<Rightarrow> bool) = strict_partial_order_on (mem_of S)"
+  unfolding strict_partial_order_on_def by simp
+
+lemma strict_partial_order_on_set_eq_strict_partial_order_on_pred_uhint [uhint]:
+  assumes "P \<equiv> mem_of S"
+  shows "strict_partial_order_on (S :: set) :: (set \<Rightarrow> set \<Rightarrow> bool) \<Rightarrow> bool \<equiv> strict_partial_order_on P"
+  using assms by simp
+
+lemma strict_partial_order_on_set_iff_strict_partial_order_on_pred [iff]:
+  "strict_partial_order_on (S :: set) (R :: set \<Rightarrow> set \<Rightarrow> bool) \<longleftrightarrow> strict_partial_order_on (mem_of S) R"
+  by simp
+
+lemma set_strict_partial_order_on_pred_iff_strict_partial_order_on_pred [iff]:
+  "strict_partial_order_on (P :: set \<Rightarrow> bool) R \<longleftrightarrow> strict_partial_order_on P (rel R)"
+  unfolding strict_partial_order_on_def by simp
+
+lemma set_strict_partial_order_on_pred_iff_strict_partial_order_on_pred_uhint [uhint]:
+  assumes "R \<equiv> rel S"
+  and "P :: set \<Rightarrow> bool \<equiv> P'"
+  shows "strict_partial_order_on P S \<equiv> strict_partial_order_on P' R"
+  using assms by simp
+
+lemma set_strict_partial_order_on_set_eq_set_strict_partial_order_on_pred [simp]:
+  "(strict_partial_order_on (S :: set) :: set \<Rightarrow> bool) = strict_partial_order_on (mem_of S)"
+  unfolding strict_partial_order_on_def by simp
+
+lemma set_strict_partial_order_on_set_eq_set_strict_partial_order_on_pred_uhint [uhint]:
+  assumes "P \<equiv> mem_of S"
+  shows "strict_partial_order_on (S :: set) :: set \<Rightarrow> bool \<equiv> strict_partial_order_on P"
+  using assms by simp
+
+lemma set_strict_partial_order_on_set_iff_set_strict_partial_order_on_pred [iff]:
+  "strict_partial_order_on (S :: set) (R :: set) \<longleftrightarrow> strict_partial_order_on (mem_of S) R"
+  by simp
+
+overloading
+  strict_partial_order_set \<equiv> "strict_partial_order :: set \<Rightarrow> bool"
+begin
+  definition "(strict_partial_order_set :: set \<Rightarrow> bool) \<equiv> strict_partial_order_on (\<top> :: set \<Rightarrow> bool)"
+end
+
+lemma strict_partial_order_set_eq_strict_partial_order_on:
+  "(strict_partial_order :: set \<Rightarrow> bool) = strict_partial_order_on (\<top> :: set \<Rightarrow> bool)"
+  unfolding strict_partial_order_set_def ..
+
+lemma strict_partial_order_set_eq_strict_partial_order_on_uhint [uhint]:
+  assumes "P \<equiv> \<top> :: set \<Rightarrow> bool"
+  shows "(strict_partial_order :: set \<Rightarrow> bool) \<equiv> strict_partial_order_on P"
+  using assms by (simp add: strict_partial_order_set_eq_strict_partial_order_on)
+
+lemma strict_partial_order_set_iff_strict_partial_order_pred [iff]: "strict_partial_order S \<longleftrightarrow> strict_partial_order (rel S)"
+  unfolding strict_partial_order_set_def by (urule refl)
+
+lemma strict_partial_order_set_iff_strict_partial_order_pred_uhint [uhint]:
+  assumes "R \<equiv> rel S"
+  shows "strict_partial_order S \<equiv> strict_partial_order R"
+  using assms by simp
+
+
+end
