HOTG/Orders/HOTG_Wellorders.thy
@@ -1,0 +1,69 @@
+\<^marker>\<open>creator "Kevin Kappelmann"\<close>
+subsubsection \<open>Well-Orders\<close>
+theory HOTG_Wellorders
+  imports
+    HOTG_Binary_Relations_Wellfounded
+    HOTG_Strict_Linear_Orders
+    Transport.Wellorders
+begin
+
+lemma wellorder_on_set_eq_wellorder_on_pred [simp]:
+  "(wellorder_on (S :: set) :: (set \<Rightarrow> set \<Rightarrow> bool) \<Rightarrow> bool) = wellorder_on (mem_of S)"
+  unfolding wellorder_on_def by simp
+
+lemma wellorder_on_set_eq_wellorder_on_pred_uhint [uhint]:
+  assumes "P \<equiv> mem_of S"
+  shows "wellorder_on (S :: set) :: (set \<Rightarrow> set \<Rightarrow> bool) \<Rightarrow> bool \<equiv> wellorder_on P"
+  using assms by simp
+
+lemma wellorder_on_set_iff_wellorder_on_pred [iff]:
+  "wellorder_on (S :: set) (R :: set \<Rightarrow> set \<Rightarrow> bool) \<longleftrightarrow> wellorder_on (mem_of S) R"
+  by simp
+
+lemma set_wellorder_on_pred_iff_wellorder_on_pred [iff]:
+  "wellorder_on (P :: set \<Rightarrow> bool) R \<longleftrightarrow> wellorder_on P (rel R)"
+  unfolding wellorder_on_def by simp
+
+lemma set_wellorder_on_pred_iff_wellorder_on_pred_uhint [uhint]:
+  assumes "R \<equiv> rel S"
+  and "P :: set \<Rightarrow> bool \<equiv> P'"
+  shows "wellorder_on P S \<equiv> wellorder_on P' R"
+  using assms by simp
+
+lemma set_wellorder_on_set_eq_set_wellorder_on_pred [simp]:
+  "(wellorder_on (S :: set) :: set \<Rightarrow> bool) = wellorder_on (mem_of S)"
+  unfolding wellorder_on_def by simp
+
+lemma set_wellorder_on_set_eq_set_wellorder_on_pred_uhint [uhint]:
+  assumes "P \<equiv> mem_of S"
+  shows "wellorder_on (S :: set) :: set \<Rightarrow> bool \<equiv> wellorder_on P"
+  using assms by simp
+
+lemma set_wellorder_on_set_iff_set_wellorder_on_pred [iff]:
+  "wellorder_on (S :: set) (R :: set) \<longleftrightarrow> wellorder_on (mem_of S) R"
+  by simp
+
+overloading
+  wellorder_set \<equiv> "wellorder :: set \<Rightarrow> bool"
+begin
+  definition "(wellorder_set :: set \<Rightarrow> bool) \<equiv> wellorder_on (\<top> :: set \<Rightarrow> bool)"
+end
+
+lemma wellorder_set_eq_wellorder_on:
+  "(wellorder :: set \<Rightarrow> bool) = wellorder_on (\<top> :: set \<Rightarrow> bool)"
+  unfolding wellorder_set_def ..
+
+lemma wellorder_set_eq_wellorder_on_uhint [uhint]:
+  assumes "P \<equiv> \<top> :: set \<Rightarrow> bool"
+  shows "(wellorder :: set \<Rightarrow> bool) \<equiv> wellorder_on P"
+  using assms by (simp add: wellorder_set_eq_wellorder_on)
+
+lemma wellorder_set_iff_wellorder_pred [iff]: "wellorder S \<longleftrightarrow> wellorder (rel S)"
+  unfolding wellorder_set_def by (urule refl)
+
+lemma wellorder_set_iff_wellorder_pred_uhint [uhint]:
+  assumes "R \<equiv> rel S"
+  shows "wellorder S \<equiv> wellorder R"
+  using assms by simp
+
+end
