HOTG/Ordinals/HOTG_Ordinals.thy
@@ -2,11 +2,11 @@
 \<^marker>\<open>creator "Kevin Kappelmann"\<close>
 theory HOTG_Ordinals
   imports
+    HOTG_Order_Types
     HOTG_Ordinals_Base
     HOTG_Ordinals_Equipollent
     HOTG_Ordinals_Max
     HOTG_Ordinals_Omega
-    HOTG_Order_Type
     HOTG_Ranks
 begin
 
