HOTG/Ordinals/HOTG_Ordinals_Equipollent.thy
@@ -4,7 +4,7 @@ theory HOTG_Ordinals_Equipollent
   imports
     HOTG_Choice
     HOTG_Equipollence_Base
-    HOTG_Transfinite_Recursion
+    HOTG_Epsilon_Recursion
     HOTG_Ordinals_Base
     HOTG_Set_Difference
 begin
@@ -15,7 +15,7 @@ text \<open>The following requires the axiom of choice. It is in fact equivalent
 over ZF since it implies the well ordering theorem.\<close>
 
 (*TODO: could be prettified using more lemmas about injective_on and the_inverse_on*)
-lemma bex_ordinal_equipollent: "\<exists>\<nu> : ordinal. X \<approx> \<nu>"
+lemma bex_ordinal_equipollent: "\<exists>\<gamma> : ordinal. X \<approx> \<gamma>"
 proof -
   (* Proof idea: form X into an ordered sequence e\<^sub>\<alpha> indexed by ordinals \<alpha> *)
   obtain f :: "set \<Rightarrow> set" where "((X : powerset X \<setminus> {\<emptyset>}) \<Rightarrow> X) f"
@@ -23,9 +23,9 @@ proof -
   then have f_mem: "f Y \<in> Y" if "Y \<subseteq> X" "Y \<noteq> \<emptyset>" for Y using that by auto
   define \<Omega> where "\<Omega> = X" (* "end of sequence" symbol *)
   let ?step = "\<lambda>e \<alpha>. if X \<setminus> {e \<beta> | \<beta> \<in> \<alpha>} \<noteq> \<emptyset> then f (X \<setminus> {e \<beta> | \<beta> \<in> \<alpha>}) else \<Omega>"
-  define e where "e = transfrec ?step"
+  define e where "e = mem_rec ?step"
   have e_eq: "e \<alpha> = ?step e \<alpha>" for \<alpha>
-    unfolding e_def using transfrec_eq[of ?step \<alpha>] repl_fun_restrict_set_eq_repl by auto
+    unfolding e_def using mem_rec_eq[of ?step \<alpha>] repl_fun_restrict_set_eq_repl by auto
   have e_mem_if_nonempty: "e \<alpha> \<in> X \<setminus> {e \<beta> | \<beta> \<in> \<alpha>}" if "X \<setminus> {e \<beta> | \<beta> \<in> \<alpha>} \<noteq> \<emptyset>" for \<alpha>
   proof -
     from that have "e \<alpha> = f (X \<setminus> {e \<gamma> | \<gamma> \<in> \<alpha>})" using e_eq[of \<alpha>] by auto
@@ -65,63 +65,63 @@ proof -
   qed
   from nr_unique have nr_e_eq_self: "nr (e \<alpha>) = \<alpha>" if "ordinal \<alpha>" "e \<alpha> \<in> Y" for \<alpha>
     using that by auto
-  define \<nu> where "\<nu> = {nr y | y \<in> Y}"
-  have e_mem_Y: "e \<alpha> \<in> Y" and nr_e_eq_self': "nr (e \<alpha>) = \<alpha>" if "\<alpha> \<in> \<nu>" for \<alpha>
+  define \<gamma> where "\<gamma> = {nr y | y \<in> Y}"
+  have e_mem_Y: "e \<alpha> \<in> Y" and nr_e_eq_self': "nr (e \<alpha>) = \<alpha>" if "\<alpha> \<in> \<gamma>" for \<alpha>
   proof -
-    from \<open>\<alpha> \<in> \<nu>\<close> obtain y where hy: "y \<in> Y" "\<alpha> = nr y" using \<nu>_def by auto
+    from \<open>\<alpha> \<in> \<gamma>\<close> obtain y where hy: "y \<in> Y" "\<alpha> = nr y" using \<gamma>_def by auto
     then show "e \<alpha> \<in> Y" using e_nr_eq_self by auto
     then show "nr (e \<alpha>) = \<alpha>" using nr_e_eq_self hy ordinal_nr by auto
   qed
   have "has_inverse_on ordinal e x" if "x \<in> X" for x
   proof -
-    obtain \<beta> where "ordinal \<beta>" "\<beta> \<notin> \<nu>" using bex_ordinal_not_mem by blast
+    obtain \<beta> where "ordinal \<beta>" "\<beta> \<notin> \<gamma>" using bex_ordinal_not_mem by blast
     have "X \<setminus> {e \<alpha> | \<alpha> \<in> \<beta>} = \<emptyset>"
     proof (rule ccontr)
       assume "X \<setminus> {e \<alpha> | \<alpha> \<in> \<beta>} \<noteq> \<emptyset>"
       then have "e \<beta> \<in> Y" using e_mem_if_nonempty \<open>ordinal \<beta>\<close> Y_def by auto
       then have "nr (e \<beta>) = \<beta>" using nr_e_eq_self \<open>ordinal \<beta>\<close> by auto
-      moreover have "nr (e \<beta>) \<in> \<nu>" using \<nu>_def \<open>e \<beta> \<in> Y\<close> by blast
-      ultimately show "False" using \<open>\<beta> \<notin> \<nu>\<close> by auto
+      moreover have "nr (e \<beta>) \<in> \<gamma>" using \<gamma>_def \<open>e \<beta> \<in> Y\<close> by blast
+      ultimately show "False" using \<open>\<beta> \<notin> \<gamma>\<close> by auto
     qed
     then obtain \<alpha> where "\<alpha> \<in> \<beta>" "x = e \<alpha>" using \<open>x \<in> X\<close> by blast
     then show ?thesis using ordinal_if_mem_if_ordinal \<open>ordinal \<beta>\<close> by blast
   qed
   then have "X = Y" unfolding Y_def by auto
-  have "bijection_on Y \<nu> nr e"
+  have "bijection_on Y \<gamma> nr e"
   proof (urule bijection_onI)
-    show "(mem_of Y \<Rightarrow> mem_of \<nu>) nr" unfolding \<nu>_def by auto
+    show "(mem_of Y \<Rightarrow> mem_of \<gamma>) nr" unfolding \<gamma>_def by auto
   qed (auto simp: e_mem_Y nr_e_eq_self' e_nr_eq_self)
-  moreover have "ordinal \<nu>"
+  moreover have "ordinal \<gamma>"
   proof (intro ordinal_if_mem_trans_closedI)
-    have "\<beta> \<in> \<nu>" if "\<alpha> \<in> \<nu>" "\<beta> \<in> \<alpha>" for \<alpha> \<beta>
+    have "\<beta> \<in> \<gamma>" if "\<alpha> \<in> \<gamma>" "\<beta> \<in> \<alpha>" for \<alpha> \<beta>
     proof -
-      have "e \<alpha> \<noteq> \<Omega>" using e_mem_Y \<open>\<alpha> \<in> \<nu>\<close> \<open>\<Omega> \<notin> Y\<close> by blast
-      have "ordinal \<alpha>" "ordinal \<beta>" using ordinal_nr \<nu>_def that ordinal_if_mem_if_ordinal by auto
+      have "e \<alpha> \<noteq> \<Omega>" using e_mem_Y \<open>\<alpha> \<in> \<gamma>\<close> \<open>\<Omega> \<notin> Y\<close> by blast
+      have "ordinal \<alpha>" "ordinal \<beta>" using ordinal_nr \<gamma>_def that ordinal_if_mem_if_ordinal by auto
       then have "\<beta> \<subseteq> \<alpha>" using \<open>\<beta> \<in> \<alpha>\<close> by (auto elim: ordinal_mem_trans_closedE)
       then have "X \<setminus> {e \<gamma> | \<gamma> \<in> \<alpha>} \<subseteq> X \<setminus> {e \<gamma> | \<gamma> \<in> \<beta>}" by blast
       moreover have "X \<setminus> {e \<gamma> | \<gamma> \<in> \<alpha>} \<noteq> \<emptyset>" using \<open>e \<alpha> \<noteq> \<Omega>\<close> e_eq[of \<alpha>] by force
       ultimately have "X \<setminus> {e \<gamma> | \<gamma> \<in> \<beta>} \<noteq> \<emptyset>" by auto
       then have "e \<beta> \<in> Y" using e_mem_if_nonempty \<open>ordinal \<beta>\<close> Y_def by auto
-      then show ?thesis unfolding \<nu>_def using nr_e_eq_self \<open>ordinal \<beta>\<close> by blast
+      then show ?thesis unfolding \<gamma>_def using nr_e_eq_self \<open>ordinal \<beta>\<close> by blast
     qed
-    then show "mem_trans_closed \<nu>" by auto
+    then show "mem_trans_closed \<gamma>" by auto
   next
-    fix \<alpha> assume "\<alpha> \<in> \<nu>"
-    then show "mem_trans_closed \<alpha>" using ordinal_nr \<nu>_def by (auto elim: ordinal_mem_trans_closedE)
+    fix \<alpha> assume "\<alpha> \<in> \<gamma>"
+    then show "mem_trans_closed \<alpha>" using ordinal_nr \<gamma>_def by (auto elim: ordinal_mem_trans_closedE)
   qed
   ultimately show ?thesis using \<open>X = Y\<close> by auto
 qed
 
-corollary wellordering_theorem: 
-  fixes X :: set
-  shows "\<exists>R :: set \<Rightarrow> set \<Rightarrow> bool. wellorder_on X R"
+text \<open>The wellordering theorem:\<close>
+
+theorem ex_rel_wellorder_on: "\<exists>(R :: set \<Rightarrow> set \<Rightarrow> bool). wellorder_on (X :: set) R"
 proof -
-  obtain \<nu> where "ordinal \<nu>" "X \<approx> \<nu>" using bex_ordinal_equipollent by blast
-  then obtain nr e :: "set \<Rightarrow> set" where "bijection_on X \<nu> nr e" by auto
-  then have "(X \<Rightarrow> \<nu>) nr" "injective_on X nr"
-    using injective_on_if_bijection_on_left mono_wrt_pred_if_bijection_on_left by auto
-  then show ?thesis
-    using wellorder_on_pullback wellorder_on_mem_if_ordinal \<open>ordinal \<nu>\<close> by blast
+  obtain \<alpha> where "ordinal \<alpha>" "X \<approx> \<alpha>" using bex_ordinal_equipollent by blast
+  then obtain nr e :: "set \<Rightarrow> set" where "bijection_on X \<alpha> nr e" by auto
+  then have "(X \<Rightarrow> \<alpha>) nr" "injective_on X nr"
+    using injective_on_if_bijection_on_left by auto
+  then show ?thesis using wellorder_on_rel_map_if_injective_on_if_mono_wrt_pred_if_wellorder_on
+    wellorder_on_mem_if_ordinal \<open>ordinal \<alpha>\<close> by blast
 qed
 
 end
