Isabelle_Set/Binary_Relations/Properties/TSBinary_Relations_Asymmetric.thy
@@ -1,0 +1,29 @@
+\<^marker>\<open>creator "Kevin Kappelmann"\<close>
+subsection \<open>Asymmetric\<close>
+theory TSBinary_Relations_Asymmetric
+  imports
+    HOTG.HOTG_Binary_Relations_Asymmetric
+    Soft_Types.Soft_Types_HOL_Base
+begin
+
+overloading
+  set_asymmetric_on_type \<equiv> "asymmetric_on :: set type \<Rightarrow> set \<Rightarrow> bool"
+begin
+  definition "set_asymmetric_on_type (T :: set type) :: set \<Rightarrow> bool \<equiv> asymmetric_on (of_type T)"
+end
+
+lemma set_asymmetric_on_type_eq_set_asymmetric_on_pred [simp]:
+  "(asymmetric_on (T :: set type) :: set \<Rightarrow> bool) = asymmetric_on (of_type T)"
+  unfolding set_asymmetric_on_type_def by simp
+
+lemma set_asymmetric_on_type_eq_set_asymmetric_on_pred_uhint [uhint]:
+  assumes "P \<equiv> of_type T"
+  shows "asymmetric_on (T :: set type) :: set \<Rightarrow> bool \<equiv> asymmetric_on P"
+  using assms by simp
+
+lemma set_asymmetric_on_type_iff_set_asymmetric_on_pred [iff]:
+  "asymmetric_on (T :: set type) (R :: set) \<longleftrightarrow> asymmetric_on (of_type T) R"
+  by simp
+
+
+end
